### Trick:
- flatten left and right subtree.
- combine (left and right subtree), cos there could be cases where one or both or none are null.
- add the result from above to root.right.

### Code 1:
```java
/**
 * Definition for a binary tree node.
 * public class TreeNode {
 *     int val;
 *     TreeNode left;
 *     TreeNode right;
 *     TreeNode() {}
 *     TreeNode(int val) { this.val = val; }
 *     TreeNode(int val, TreeNode left, TreeNode right) {
 *         this.val = val;
 *         this.left = left;
 *         this.right = right;
 *     }
 * }
 */
class Solution {
    private TreeNode[] combine(TreeNode[] lft, TreeNode[] rgt){
        TreeNode[] ans = new TreeNode[2]; 
        if(lft[0]==null && rgt[0]==null){
            return lft;
        }else if(lft[0]==null){
            return rgt;
        }else if(rgt[0]==null){
            return lft;
        }

        lft[1].right = rgt[0];
        ans[0] = lft[0];
        ans[1] = rgt[1];
        return ans;
    }

    private TreeNode[] fcn(TreeNode root) {
        TreeNode[] ans = new TreeNode[2];
        if(root==null){
            ans[0] = ans[1] = null;
            return ans;
        }

        TreeNode[] lft = fcn(root.left);
        TreeNode[] rgt = fcn(root.right);
        TreeNode[] pt = combine(lft, rgt);
        root.right = pt[0];
        root.left = null;
        ans[0] = root;
        ans[1] = (pt[1]==null)?(root):(pt[1]);
        return ans;
    }

    public void flatten(TreeNode root) {

        TreeNode[] ans = new TreeNode[2];
        ans = fcn(root);
    }
}
```

### Code 2:
```java
/**
 * Definition for a binary tree node.
 * public class TreeNode {
 *     int val;
 *     TreeNode left;
 *     TreeNode right;
 *     TreeNode() {}
 *     TreeNode(int val) { this.val = val; }
 *     TreeNode(int val, TreeNode left, TreeNode right) {
 *         this.val = val;
 *         this.left = left;
 *         this.right = right;
 *     }
 * }
 */
class Solution {
    private TreeNode get(TreeNode root){
        if(root==null || (root.left==null && root.right==null)){
            return root;
        }else if(root.left==null){
            TreeNode temp = get(root.right);
            temp.left = temp.right = null;
            return temp;
        }else if(root.right==null){
            TreeNode temp = get(root.left);
            root.right = root.left;
            root.left = null;
            temp.left = temp.right = null;
            return temp;
        }else{
            TreeNode temp1 = get(root.left);
            TreeNode temp2 = get(root.right);
            temp1.right = root.right;
            root.right = root.left;
            root.left = null;
            temp2.left = temp2.right = null;
            return temp2;
        }
    }
    public void flatten(TreeNode root) {
        TreeNode xx = get(root);
    }
}
```